Želimo, da je vsota Gibalnih količin in Kinetičnih energij pred in po trku enaka.

Gibalna količina: $p = m*v \ [\frac{kg \ m}{s}]$
Kinetična energija: $W_{k}=\frac{m \ v^2}{2} \ [J] \ [\frac{m^3}{s^2}]$

$$\text{Gibalna količina:}$$
$$p_{Ai} + p_{Bi}=p_{Af}+p_{Bf}$$
$$m_{A}*v_{Ai}+m_{B}*v_{Bi}=m_{A}*v_{Af}+m_{B}*v_{Bf}$$

$$\text{Kinetična energija}$$
$$W_{kAi} + W_{kBi} = W_{kAf} + W_{kBf}$$
$$\frac{m_{A} \ v_{Ai}^2}{2}+ \frac{m_{B} \ v_{Bi}^2}{2} = \frac{m_{A} \ v_{Af}^2}{2} + \frac{m_{B} \ v_{Bf}^2}{2}$$
---
$$\text{Obe neznanki } v_{Af} \text{ in } v_{Bf} \text{ lahko zdaj rešimo saj imamo dve enačbi}$$
$$m_{A}*v_{Ai}+m_{B}*v_{Bi}=m_{A}*v_{Af}+m_{B}*v_{Bf}$$
$$m_{A}*v_{Ai} - m_{A}*v_{Af}=m_{B}*v_{Bf} - m_{B}*v_{Bi}$$
$$\underline{\underline{m_{A}(v_{Ai}-v_{Af})=m_{B}(v_{Bf}-v_{Bi})}}$$
$$\frac{1}{2}m_A v_{Ai}^2+\frac{1}{2}m_B v_{Bi}^2=\frac{1}{2}m_A v_{Af}^2+\frac{1}{2}m_B v_{Bf}^2$$
$$m_A ( v_{Ai}^2 - v_{Af}^2 ) = m_B ( v_{Bf}^2-v_{Bi}^2)$$
$$\underline{\underline{m_A (v_{Ai} – v_{Af})(v_{Ai} + v_{Af}) = m_B(v_{Bf} – v_{Bi})(v_{Bf} + v_{Bi})}}$$
$$\frac{m_A (v_{Ai} - v_{Af}) (v_{Ai} + v_{Af})}{m_A (v_{Ai} - v_{Af})} = \frac{m_B (v_{Bf} - v_{Bi}) (v_{Bf} + v_{Bi})}{m_B (v_{Bf} - v_{Bi})}$$
$$\underline{\underline{v_{Ai} + v_{Af} = v_{Bf} + v_{Bi}}}$$
$$v_{Bf}=v_{Ai}+v_{Af}-v_{Bi}$$
$$m_{A}​*v_{Af}​=m_{A}​*v_{Ai}​+m_{B​}*v_{Bi}​−m_B​(v_{Ai}​+v_{Af​}−v_{Bi}​)$$
$$m_B (v_{Ai} + v_{Af} - v_{Bi}) = m_B v_{Ai} + m_B v_{Af} - m_B v_{Bi}$$
$$\begin{aligned}
 m_A v_{Af} &= m_A v_{Ai} + m_B v_{Bi} - m_B(v_{Ai}+v_{Af}-v_{Bi}) \\
                       m_A v_{Af} &= m_A v_{Ai} + m_B v_{Bi} - m_B v_{Ai} - m_B v_{Af} + m_B v_{Bi}\\
 m_A v_{Af} + m_B v_{Af} &= m_A v_{Ai} + m_B v_{Bi} - m_B v_{Ai} + m_B v_{Bi}\end{aligned}$$
 $$(m_A + m_B) v_{Af} = (m_A-m_B)v_{Ai} + 2m_B v_{Bi}$$
$$ \boxed{v_{Af} = \left( \frac{m_{A}-m_{B}}{m_{A}+m_{B}} \right) v_{Ai} + \left( \frac{2m_{B}}{m_{A}+m_{B}} \right) v_{Bi}} $$ $$\begin{aligned} v_{Bf} &= v_{Ai}+v_{Af}-v_{Bi}\\
&= v_{Ai} + \left( \frac{m_{A}-m_{B}}{m_{A}+m_{B}} \right) v_{Ai} + \left( \frac{2m_{B}}{m_{A}+m_{B}} \right) v_{Bi}-v_{Bi} \end{aligned}$$
$$v_{Bf} = \frac{(m_A + m_B)+(m_A - m_B)}{m_A + m_B} v_{Ai} + \frac{2m_B-(m_A+m_B)}{m_A + m_B} v_{Bi}$$
$$\boxed{v_{Bf} = \left( \frac{2m_{A}}{m_{A}+m_{B}} \right) v_{Ai} +  \left( \frac{m_{B}-m_{A}}{m_{A}+m_{B}} \right) v_{Bi}}$$