$$c^2=a^2*(ka)^2-2\cos\gamma *a * ka$$ $$c^2=a^2*k^2*a^2-2\cos\gamma *k*a^2$$ $$c^2=a^2*(1+k^2-2k*\cos\gamma)$$ $$a^2=c^2*(1+k^2-2k*\cos\gamma)$$ $$\underline{\underline{a=\sqrt{ \frac{c^2}{1+k^2+2k*\cos\gamma} }}}$$ $$\textbf{skalarni produkt:}$$ $$|v_1| * |v_2| * \cos(\alpha) = x_1 \cdot x_2 + y_1 \cdot y_2$$$$ \cos(\alpha) = \frac{x_1 \cdot x_2 + y_1 \cdot y_2}{|v_1| |v_2|} $$$$\cos^2(\alpha) = \left( \frac{x_1 \cdot x_2 + y_1 \cdot y_2}{|v_1| |v_2|} \right)^2 $$$$|v| = \sqrt{x^2 + y^2} $$$$\cos^2(\alpha) = \frac{(x_1 \cdot x_2 + y_1 \cdot y_2)^2}{(x_1^2 + y_1^2)(x_2^2 + y_2^2)} $$

---
$$\underline{\underline{a=\sqrt{ \frac{c^2}{1+k^2+2k*\sqrt{\frac{(x_1 \cdot x_2 + y_1 \cdot y_2)^2}{(x_1^2 + y_1^2)(x_2^2 + y_2^2)}}}}}}$$ $$b = k*a$$ --- 
$$t=\frac{a}{\sqrt{ x_{i}^2 + y_{i}^2}}$$ $$t=\frac{b}{\sqrt{ x_{f}^2 + y_{f}^2}}$$ $$\frac{b}{\sqrt{ x_{f}^2 + y_{f}^2}}=\frac{a}{\sqrt{ x_{i}^2 + y_{i}^2}}$$$$b=\frac{a * \sqrt{ x_{f}^2 + y_{f}^2}}{\sqrt{ x_{i}^2 + y_{i}^2}}$$ $$b^2=\frac{a^2 * (x_{f}^2 + y_{f}^2)}{( x_{i}^2 + y_{i}^2)}$$ $$b=\sqrt{\frac{a^2 * (x_{f}^2 + y_{f}^2)}{( x_{i}^2 + y_{i}^2)}}$$ $$x_{v}=x_{i}-v_{ix}*t$$ $$x_{f}=x_{v}+v_{fx}*t$$ $$x_{f}=x_{i}-v_{ix}*t+v_{fx}*t$$ $$x_{f}=x_{i}+ t*(v_{fx}-v_{ix})$$ $$y_{f}=y_{i}+ t*(v_{fy}-v_{iy})$$