$$(\sin x)'=\cos x$$
$$(\cos x)'=(\sin(\frac{\pi}{2}  -x))'=\cos(\frac{\pi}{2}-x)*(-1) = -\sin x$$
$$(\tan x)'=(\frac{\sin x}{\cos x})'= \frac{\cos x*\cos x-\sin x(-\sin x)}{\cos^2x}=\frac{\cos^2x+\sin^2x}{\cos^2x}=\frac{1}{\cos^2x}$$
$$(\cot x)'=(\frac{\cos x}{\sin x})'=\frac{-\sin x* \sin x-\cos x*\cos x}{\sin^2x}= -\frac{1}{\sin^2x}$$
---
$$(\arcsin x)' = \frac{1}{\sqrt{1-x^2}}$$
$$(\arccos x)' = - \frac{1}{\sqrt{1-x^2}}$$
$$(\arctan x)' = \frac{1}{1+x^2}$$
$$(\arccos x)'=-\frac{1}{1+x^2}$$
---
$$(\arcsin x)'$$
$$\sin(\arcsin x)= x$$
$$\cos(\arcsin x)*(\arcsin x)' = 1$$
$$(\arcsin x)'=\frac{1}{\sqrt{1-\sin^2(\arcsin x)}} = \frac{1}{\sqrt{1-\sin^2(\arcsin x)}}$$
$$\tan(\arctan x) = x$$
$$\frac{1}{\cos^2(\arctan x)}*(\arctan x)' = 1$$
$$(\arctan x)'=\cos^2(\arctan x) = 1 + \tan^2x=\frac{1}{\cos^2x} = \frac{1}{1 + \tan^2(\arctan x)} = \frac{1}{1 + x^2}$$

