Odvod konstante je 0.
Odvod vsote oz razlike funkcij:
$$(f+g)'(x) = f'(x) \pm g'(x)$$
$$(x^2-x+3)'=2x-1$$
odvod produkta dveh funkcij:
$$(f*g)'(x)=f'(x)*g(x) + f(x)*g'(x)$$
$$(x^4)'=(x^2*x^2)'=2x*x^2+x^2*2x = 4x^3$$
$$(x^5)'=(x^2*x^3)'=2x*x^3+x^2*3x^2=5x^4$$
$$(x^n)'=nx^{n-1} \qquad n \in \mathbb{N}$$
Odvod produkta konstante in funkcije:
$$k \in \mathbb{R} \qquad (k*f)'(x) = k*f'(x)$$

Odvod koliƒçnika
$$(\frac{f}{g})'=\frac{f'*g-f*g'}{g^2}$$

$$(x^{-n})'=(\frac{1}{x^n})'=\frac{1'*x^n-1*n*x^{n-1}}{x^{2n}}=\frac{-nx^{n-1}}{x^{2n}}=-nx^{-n-1}$$

