$S_n = a_1 + \dots + a_n = \frac{a_1(k^n - 1)}{k - 1}$
$\lim_{n \to \infty} S_n = \lim_{n \to \infty} \frac{a_1(k^n - 1)}{k - 1}$

$|k| \geq 1$: $S$ ne obstaja
$|k| < 1$: $S = \frac{- a_1}{k - 1}$
$\underline{\underline{S = \frac{a_1}{1 - k}}}$

$1 + \frac{1}{2} + \frac{1}{4} + \dots = \frac{a_1}{1 - k} = \frac{1}{\frac{1}{2}} = 2$
$2 + \frac{2}{3} + \frac{2}{9} + \dots = \frac{2}{1 - \frac{1}{3}} = \frac{2}{\frac{2}{3}} = 3$
$1 - \cos \alpha + \cos \frac{1}{\alpha} - \cos^3 \alpha = \frac{1}{1 + \cos \alpha}$