Izjava, ki jo dokazujemo za vsa $\mathbb{N}$ števila.
1. Dokažemo, da velja za $n = 1$
2. Iz predpostavke, da velja za $n$, dokažemo, da velja za $n + 1$.
---
$$1 + 2 + 3 + \dots + n = \frac{n(n + 1)}{2}$$

1. $$n = 1: \quad \frac{1 * (1 + 1)}{2} = \frac{2}{2} = 1$$
2. $$\underline{\underline{S_n + a_{n + 1} = S_{n + 1}}}$$
$$S_n + a_{n + 1} = \frac{n(n + 1)}{2} + n + 1 = \frac{n^2 + n + 2n + 2}{2} = \frac{n^2 + 3n + 2}{2} = \underline{\underline{\frac{(n + 1)(n + 2)}{2}}}$$
$$S_{n + 1} = \frac{(n + 1)((n + 1) + 1)}{2} = \underline{\underline{\frac{(n + 1)(n + 2)}{2}}}$$