Funkciji $f(x)$ in $f^{-1}(x)$: $f^{-1}(f(x))=x$ in $f(f^{-1}(x))=x$
$(f(x))^{-1}=\frac{1}{f(x)}$
Primeri:
$a^x$, $\log_a x$
$x^{2n-1}$, $\sqrt[2n-1]{x}$
$x^{2n}=\sqrt[2n]{x} \rightarrow [0, \infty)$
$\sin x$, $\arcsin x \rightarrow [-\frac{\pi}{2}, \frac{\pi}{2}]$


$f(x)=2x+1$
$f^{-1}=\frac{x-1}{2}$
```functionplot
---
title: 
xLabel: 
yLabel: 
bounds: [-10,10,-10,10]
disableZoom: false
grid: true
---
f(x)=2x+1
f^{-1}(x)=(x-1)/2
s(x)=x
```

$f(x)=\frac{x-1}{x}$
$D_f=\mathbb{R} - {0}$
$f^{-1}(x)=\frac{1}{x-1}$
$D_{f^{-1}}=\mathbb{R} - {1}$

```functionplot
---
title: 
xLabel: 
yLabel: 
bounds: [-10,10,-10,10]
disableZoom: false
grid: true
---
f(x)=(x-1)/x
f'(x)=1/x-1
```
$f(x)=x^2-1$, $x \leq 0$
$y=x^2-1$
$x=-\sqrt{y+1}$
$f^{-1}(x)=-\sqrt{y+1}$


$f(x)=\ln(x+3)-1$
$D_f=(-3, \infty)$
$f'(x)=e^{x+1}-3$

$f(x)=3^{2-x}+1$
$y-1=3^{2-x}$
$\log_3 (y-1) = 2 -x$
$x=-\log_3 (y-1) +2$
$D_f = (1, \infty)$

$f(x)=\arcsin (2x-1)$
$y=\frac{\sin x + 1}{2}$

